Start on proof that reverse uses constant stack space

examples/cost/reverseProofScript.sml
@@ -17,4 +17,142 @@ val reverse_x64_conf = (rand o rator o lhs o concl) reverse_thm
 val _ = install_naming_overloads "reverseProg";
 val _ = write_to_file reverse_data_prog_def;
 
+val reverse_body =
+  “lookup_reverse (fromAList reverse_data_prog)”
+  |> (REWRITE_CONV [reverse_data_prog_def] THENC EVAL)
+  |> concl |> rand |> rand |> rand
+
+Definition repchar_list_def:
+  (* cons *)
+  (repchar_list (Block ts _ [Number i; rest]) (l:num) (tsb:num) ⇔
+    (0 ≤ i ∧ i ≤ 255 ∧ (* i reps a character *)
+    ts < tsb ∧
+    l > 0 ∧ repchar_list rest (l-1) tsb)) ∧
+  (* nil *)
+  (repchar_list (Block _ tag []) (l:num) tsb ⇔ (tag = 0)) ∧
+  (* everything else *)
+  (repchar_list _ _ _ ⇔ F)
+End
+
+Theorem reverse_code_constant_stack:
+  ∀s ts sstack lsize res s'.
+   s.safe_for_space ∧
+   wf s.refs ∧
+   (s.stack_frame_sizes = reverse_config.word_conf.stack_frame_size) ∧
+   (size_of_stack s.stack = SOME sstack) ∧
+   (s.locals_size = SOME lsize) ∧
+   s.limits.arch_64_bit ∧
+   closed_ptrs (stack_to_vs s) s.refs ∧
+   2 ≤ s.limits.length_limit ∧
+   (s.tstamps = SOME ts) ∧
+   0 < ts ∧
+   (s.locals = fromList [block]) ∧
+   (repchar_list block l ts) ∧
+   (s.code = fromAList reverse_data_prog) ∧
+   (evaluate (^reverse_body, s) = (res,s'))
+   ⇒ ∃k. s'.stack_max = OPTION_MAP ($+ k) s.stack_max
+Proof
+ let
+  val code_lookup   = mk_code_lookup
+                        `fromAList reverse_data_prog`
+                         reverse_data_code_def
+  val frame_lookup   = mk_frame_lookup
+                        `reverse_config.word_conf.stack_frame_size`
+                         reverse_config_def
+  val strip_assign  = mk_strip_assign code_lookup frame_lookup
+  val yk_strip_assign  = qmatch_goalsub_abbrev_tac `bind _ rest_ass _`
+  \\ ASM_REWRITE_TAC [ bind_def           , assign_def
+                     , op_space_reset_def , closLangTheory.op_case_def
+                     , cut_state_opt_def  , option_case_def
+                     , do_app_def         , data_spaceTheory.op_space_req_def
+                     , do_space_def       , closLangTheory.op_distinct
+                     , MEM                , IS_NONE_DEF
+                     , add_space_def      , check_lim_def
+                     , do_stack_def       , flush_state_def
+                     , cut_state_def
+                     , bvi_to_dataTheory.op_requires_names_eqn ]
+  \\ BETA_TAC
+  \\ TRY(eval_goalsub_tac ``dataSem$cut_env _ _`` \\ simp [])
+  \\ TRY(eval_goalsub_tac ``dataSem$get_vars    _ _`` \\ simp [])
+  \\ simp [ do_app_aux_def    , set_var_def       , lookup_def
+          , domain_IS_SOME    , code_lookup       , size_of_heap_def
+          , consume_space_def , with_fresh_ts_def , stack_consumed_def
+          , frame_lookup      , allowed_op_def    , size_of_stack_def
+          , flush_state_def   , vs_depth_def      , eq_code_stack_max_def
+          , lookup_insert     , semanticPrimitivesTheory.copy_array_def
+          , size_of_stack_frame_def
+          , backend_commonTheory.small_enough_int_def ]
+  \\ (fn (asm, goal) => let
+        val pat   = ``sptree$lookup _ _``
+        val terms = find_terms (can (match_term pat)) goal
+        val simps = map (PATH_CONV "lr" EVAL) terms
+      in ONCE_REWRITE_TAC simps (asm,goal) end)
+  \\ simp [frame_lookup]
+  \\ Q.UNABBREV_TAC `rest_ass`                                                  
+  val open_call     = mk_open_call code_lookup frame_lookup
+  val make_call     = mk_make_call open_call
+  val strip_call    = mk_strip_call open_call
+  val open_tailcall = mk_open_tailcall code_lookup frame_lookup
+  val make_tailcall = mk_make_tailcall open_tailcall
+  in
+  measureInduct_on `^s.clock`
+  \\ fs [ to_shallow_thm
+        , to_shallow_def
+        , initial_state_def ]
+  \\ rw [] \\ fs [fromList_def]
+  \\ pop_assum mp_tac
+  \\ yk_strip_assign
+  \\ rename1 `state_safe_for_space_fupd (K safe) _`
+  \\ yk_strip_assign
+  \\ TOP_CASE_TAC >> fs[repchar_list_def]
+  \\ reverse TOP_CASE_TAC >-
+     (rw[] >> fs[AllCaseEqs()] >> rveq >> rw[] >>
+      Cases_on ‘s.stack_max’ >> rw[MAX_DEF] >> intLib.COOPER_TAC)
+  \\ simp[Once bind_def,data_monadTheory.if_var_def,lookup_insert]
+  \\ TOP_CASE_TAC >-
+     (rw[] >> fs[AllCaseEqs()] >> rveq >> rw[] >>
+      Cases_on ‘s.stack_max’ >> rw[MAX_DEF] >> intLib.COOPER_TAC)
+  \\ fs[CaseEq "dataSem$v",CaseEq "prod", CaseEq "option", CaseEq "semanticPrimitives$result"] >> rveq >> fs[] >> rveq >> fs[]
+  \\ IF_CASES_TAC >-
+     (yk_strip_assign >>
+      qmatch_goalsub_abbrev_tac ‘if a1 then _ else _’ >>
+      ‘a1’ by(qunabbrev_tac ‘a1’ >> EVAL_TAC) >>
+      simp[] >>
+      qunabbrev_tac ‘a1’ >>
+      simp[get_vars_def,get_var_def,lookup_inter,lookup_def,lookup_insert] >>
+      simp[v_to_list_def,backend_commonTheory.nil_tag_def] >>
+      simp[flush_state_def,check_lim_def] >>
+      rw[] >> simp[] >>
+      Cases_on ‘s.stack_max’ >> rw[PULL_EXISTS] >>
+      simp[reverse_config_def,lookup_def] >>
+      fs[size_of_stack_def] >>
+      rw[MAX_DEF] >>
+      intLib.COOPER_TAC)
+  \\ reverse TOP_CASE_TAC >-
+     (rw[] >> fs[AllCaseEqs()] >> rveq >> rw[] >>
+      Cases_on ‘s.stack_max’ >> rw[MAX_DEF] >> intLib.COOPER_TAC)
+  \\ rename1 `state_safe_for_space_fupd (K safe') _`
+  \\ strip_makespace
+  \\ strip_assign
+  \\ strip_assign
+  \\ reverse IF_CASES_TAC >-
+     (rw[] >> fs[AllCaseEqs()] >> rveq >> rw[] >>
+      Cases_on ‘s.stack_max’ >> rw[MAX_DEF] >> intLib.COOPER_TAC)
+  \\ simp[]
+  \\ strip_assign
+  \\ strip_assign
+  \\ simp[]
+  \\ reverse IF_CASES_TAC >-
+     (rw[] >> fs[AllCaseEqs()] >> rveq >> rw[] >>
+      Cases_on ‘s.stack_max’ >> rw[MAX_DEF] >> intLib.COOPER_TAC)
+  \\ simp[]
+  \\ strip_assign
+  \\ strip_assign
+  \\ strip_assign
+  \\ simp[v_to_list_def,backend_commonTheory.cons_tag_def,backend_commonTheory.nil_tag_def]
+  \\ simp[]
+  \\ cheat
+  end
+QED
+
 val _ = export_theory();
